\begin{frame}{SecFprUrsh}

%
%
%
\iffalse
Given 64-bit shares $(x_i)$ and 6-bit shares $(c_i)$, we need to derive shares $(z_i)$ such that
\[
\bigoplus_{i=1}^n z_i = \left( \left( \bigoplus_{i=1}^n x_i \right) \gg \left( \sum_{i=1}^n c_i \bmod 2^{6} \right) \right) \vee \left \llbracket \bigoplus_{i=1}^n x_i^{[c:1]} \neq 0 \right \rrbracket
\]
%
%
%
\fi

Given 64-bit shares $(x_i)$ and 6-bit shares $(c_i)$, we need to derive shares $(z_i)$ such that
\[
\bigoplus_{i=1}^n z_i = \left( \bigoplus_{i=1}^n x_i \right) \gg \left( \sum_{i=1}^n c_i \bmod 64 \right)
\]

\pause
\medskip

We observe that
\pause
\begin{itemize}

\item Right-shifting and right-rotating by a value $c$ only differ by the most $c$ significant bits.
\pause
\item Right-rotating $x$ by a value $c$ is equal to right-rotating $x$ by $c \bmod 64$.
\end{itemize}

\end{frame}


\begin{frame}{SecFprUrsh}

Hence, our idea is to right-rotate all $x_i's$ by $c_1, c_2, \cdots, c_n$ sequentially.
\pause
\medskip

Some high bits are redundant, so we use an index $m = (1 \ll 63)$ to indicate the first meaningful bit of the result.
\pause
Consider
\[
m \gg c = (\underbrace{0 \cdots 0}_{c \text{ bits}} 1 0 \cdots 0)_2
\]
\pause
\[
m' := m \gg c \oplus (m \gg c) \gg 1 \oplus \cdots \oplus (m \gg c) \gg 63 = (\underbrace{0 \cdots 0}_{c \text{ bits}} 1 1 \cdots 1)_2
\]
\pause
By an AND operation with $m'$, we can clear useless bits.

\end{frame}


%
%
%
\iffalse

\begin{frame}{SecFprUrsh}

\centerline{
\blockalgstart{.9\textwidth}{{\large SecFprUrsh}}
\begin{algorithm}[H]
  \label{alg:SecFprUrsh}
  \algsetup{linenosize=\small}
  \small
  \begin{multicols}{2}
  \begin{algorithmic}[1]
    \REQUIRE 64-bit Boolean shares ${(x_i)_{1\leq i \leq n}}$
    \REQUIRE 6-bit arithmetic shares ${(c_i)_{1\leq i \leq n}}$
    \ENSURE Boolean shares ${(z_i)_{1\leq i \leq n}}$ for value $z = x \gg c$ with the sticky bit preserved
    \STATE ${(m_i)_{1\leq i \leq n}} \gets ((1 \ll 63), 0, \cdots, 0)$
    \FOR{$j = 1$ to $n$}
        \STATE Right-rotate $(x_i)$ by $c_j$
        \STATE $(x_i) \gets {\sf RefreshMasks}((x_i))$
        \STATE Right-rotate $(m_i)$ by $c_j$
        \STATE $(m_i) \gets {\sf RefreshMasks}((m_i))$
    \ENDFOR
    \STATE ${\sf len} \gets 1$
    \WHILE{${\sf len} \leq 32$}
        \STATE $(m_i) \gets (m_i \oplus (m_i \gg {\sf len}))$
        \STATE ${\sf len} \gets {\sf len} \ll 1 $
    \ENDWHILE
    \STATE $(y_i) \gets {\sf SecAnd}( (x_i), (m_i) )$
    \STATE $(z_i) \gets (y_i \oplus x_i \oplus y_i^{(1)})$
    \STATE $(b_i) \gets {\sf SecNonzero}( (z_i) )$
    \STATE $(z_i) \gets  (y_i^{[64:2]} \vee b_i) $
    \STATE \Return $(z_i)$
\end{algorithmic}
\end{multicols}
\end{algorithm}
\vspace{-10pt}
\blockalgend
}

\end{frame}


\begin{frame}{SecFprUrsh in Masking FprAdd}

\centerline{
\blockalgstart{.8\textwidth}{{\large FprAdd}}
\begin{algorithm}[H]
  \algsetup{linenosize=\small}
  \begin{multicols}{2}
  \small
  \begin{algorithmic}[1]
    \REQUIRE FPNs $x$ and $y$
    \ENSURE FPN sum of $x$ and $y$
    \STATE $d \gets x^{[63:1]} - y^{[63:1]}$
    \STATE $cs \gets d^{(64)} \vee ((1 - (-d)^{(64)}) \wedge x^{(64)}) $
    \STATE $m \gets (x \oplus y) \wedge (-cs)$
    \STATE $x \gets x \oplus m, y \gets y \oplus m$
    \STATE Extract $(sx, ex, mx)$ and $(sy, ey, my)$ from $x, y$, respectively.
    \STATE $mx \gets mx \ll 3, my \gets my \ll 3$
    \STATE $ex \gets ex - 1078, ey \gets ey - 1078$
    \STATE $c \gets ex - ey$
    \STATE $b \gets \llbracket c < 60 \rrbracket$ 
    \STATE $my \gets my \wedge (-b) $ 
    \STATE \textcolor{red}{$my \gets (my \gg c) \vee \llbracket my^{[c:1]} \neq 0 \rrbracket$}
    \STATE $s \gets sx \oplus sy$
    \STATE $z \gets mx + (-1)^s my $
    \STATE Normalize $z, ex$ to make the 64th bit of $z$ set
    \STATE $z \gets (z \gg  9) \vee \llbracket z^{[9:1]} \neq 0 \rrbracket$
    \STATE $ex \gets ex + 9$ \\
    \RETURN \hskip -4pt ${\sf FPR}(sx, ex, z)$
  \end{algorithmic}
  \end{multicols}
\end{algorithm}
\vspace{-10pt}
\blockalgend
}

\end{frame}

\fi